more

Systems/Protocol.v
@@ -1,4 +1,4 @@
-From Coq Require Import Bool List.
+From Coq Require Import Bool List PeanoNat Lia.
 From Coq Require ssrbool ssreflect.
 Import (coercions) ssrbool.
 Import ssreflect.SsrSyntax.
@@ -13,6 +13,46 @@ Parameter t0 : nat.
 Axiom t0_lt_N : t0 < N.
 
 End ByzThreshold.
+
+Module Type ClassicByzThreshold (Export A : NetAddr) <: ByzThreshold A.
+
+(* TODO is it possible to make this function work over arbitrary integer parameter?
+    do not quite want to introduce another module type ... *)
+
+Definition t0 := (N - 1) / 3.
+
+Fact N_gt_0 : 0 < N.
+Proof. 
+  unfold N. 
+  pose proof (Address_is_finite Address_inhabitant).
+  destruct valid_nodes; [ contradiction | simpl; apply Nat.lt_0_succ ].
+Qed.
+
+Fact t0_times_3_lt_N : 3 * t0 < N.
+Proof.
+  unfold t0, lt.
+  (* nia does not work here *)
+  pose proof N_gt_0.
+  destruct N as [ | N ]; [ inversion H | ].
+  rewrite Nat.sub_succ, Nat.sub_0_r.
+  apply le_n_S, Nat.Div0.mul_div_le.
+Qed.
+
+Fact t0_lt_N_minus_2t0 : t0 < N - (t0 + t0).
+Proof. pose proof t0_times_3_lt_N; lia. Qed.
+
+Fact t0_lt_N : t0 < N.
+Proof. pose proof t0_times_3_lt_N. lia. Qed.
+
+(* TODO some quorum-related things *)
+
+End ClassicByzThreshold.
+
+Module ClassicByzThresholdImpl (Export A : NetAddr) <: ClassicByzThreshold A <: ByzThreshold A.
+
+Include ClassicByzThreshold A.
+
+End ClassicByzThresholdImpl.
 
 Module Type Protocol (Export A : NetAddr) (Export M : MessageType) (Export P : PacketType)
   (Export BTh : ByzThreshold A).
